fixed option monad to be a record. added fuel which is generic to a monad error with a gas error injection.

theories/Monad/Monad.v
@@ -65,3 +65,9 @@ Class Zero (m : Type -> Type) : Type :=
 
 Class MonadFix (m : Type -> Type) : Type :=
 { mfix : forall {T U}, ((T -> m U) -> T -> m U) -> T -> m U }.
+
+Class Error e (m:Type->Type) :=
+{ throw : forall {A}, e -> m A
+; catch : forall {A}, m A -> (e -> m A) -> m A
+}.
+
