theories/Functional/Fun.v
@@ -5,6 +5,16 @@ Require Import Monad.Folds.
 Set Implicit Arguments.
 Set Strict Implicit.
 
+Module FunNotation.
+
+  Notation "f $ x" := (f x)
+    (at level 99, x at level 99, right associativity, only parsing).
+
+  Notation "'begin' e1 'end'" := ((e1))
+    (at level 0, only parsing).
+
+End FunNotation.
+
 Definition compose A B C (g:B -> C) (f:A -> B) (x:A) : C := g (f x).
 
 Definition forEach A B (xs:list A) (f:A -> B) : list B := map f xs.
@@ -12,12 +22,29 @@ Definition forEach A B (xs:list A) (f:A -> B) : list B := map f xs.
 Definition forEachM {m} {M:Monad m} {A B} (xs:list A) (f:A -> m B) : m (list B) :=
   mapM f xs.
 
-Module FunNotation.
+Section MonadFixDefs.
+  Context {m} {mFix:MonadFix m}.
 
-  Notation "f $ x" := (f x)
-    (at level 99, x at level 99, right associativity, only parsing).
+  Definition mfix2 {A B C}
+    (ff:(A -> B -> m C) -> (A -> B -> m C)) (a:A) (b:B) : m C :=
+      let ff' fabp (abp:A*B) :=
+        let (a,b) := abp in
+        let fab a b := fabp (a,b) in
+        ff fab a b
+      in
+      mfix ff' (a,b)
+  .
 
-  Notation "'begin' e1 'end'" := (e1)
-    (at level 0, only parsing).
+  Definition mfix3 {A B C D}
+    (ff:(A -> B -> C -> m D) -> (A -> B -> C -> m D))
+    (a:A) (b:B) (c:C) : m D :=
+      let ff' fabcp (abcp:A*B*C) :=
+        let (abp,c) := abcp in
+        let (a,b) := abp in
+        let fabc a b c := fabcp (a,b,c) in
+        ff fabc a b c
+      in
+      mfix ff' (a,b,c)
+  .
+End MonadFixDefs.
 
-End FunNotation.
