theories/Monad/Fuel.v
@@ -1,0 +1,44 @@
+Require Import Monad.
+Require Import OptionMonad.
+Require Import Undefined.
+Require Import Fun.
+
+Set Implicit Arguments.
+Set Strict Implicit.
+
+Import MonadNotationX.
+Import FunNotation.
+
+Module GasError.
+  Class HasGasError e := { gasError : e}.
+  Instance UnitHasGasError : HasGasError unit := { gasError := tt }.
+End GasError.
+
+Import GasError.
+
+Inductive fuel (m:Type->Type) A := mkFuel { unFuel : nat -> m A }.
+Implicit Arguments mkFuel [m A].
+
+Section FuelFix.
+  Context {m} {e} {mError:Error e m} {eHasGasError:HasGasError e}.
+
+  Fixpoint fuelFix' {A B:Type}
+    (ff:(A -> fuel m B) -> (A -> fuel m B)) (k:nat) (a:A) {struct k} : m B :=
+      match k with
+      | O => throw gasError
+      | S k' => unFuel (ff (fun a' => mkFuel (fun _k => fuelFix' ff k' a'))
+                           a)
+                       k'
+      end
+  .
+
+  Definition fuelFix {A B:Type}
+    (ff:(A -> fuel m B) -> (A -> fuel m B)) (a:A) : fuel m B :=
+      mkFuel (fun k => fuelFix' ff k a)
+  .
+
+  Instance FuelFixMonad : MonadFix (fuel m) :=
+    { mfix _A _B := fuelFix }
+  .
+
+End FuelFix.
